proof for `if` at level `0`
Signed-off-by: John Kastner <jkastner@amazon.com>

cedar-lean/Cedar/Validation/Levels.lean
@@ -15,6 +15,7 @@
 -/
 
 import Cedar.Validation.TypedExpr
+import Cedar.Validation.Typechecker
 
 /-!
 This file defines a level checking of a type-annotated AST. Level checking
@@ -29,44 +30,48 @@ namespace Cedar.Validation
 open Cedar.Data
 open Cedar.Spec
 
-def typedAtLevel (tx : TypedExpr) (n : Nat) : Bool :=
+def checkLevel (tx : TypedExpr) (n : Nat) : Bool :=
   match tx with
   | .lit _ _
   | .var _ _ => true
   | .ite x₁ x₂ x₃ _ =>
-    (typedAtLevel x₁ n) &&
-    (typedAtLevel x₂ n) &&
-    (typedAtLevel x₃ n)
+    (checkLevel x₁ n) &&
+    (checkLevel x₂ n) &&
+    (checkLevel x₃ n)
   | .unaryApp _ x₁ _ =>
-    typedAtLevel x₁ n
+    checkLevel x₁ n
   | .binaryApp .mem x₁ x₂ _
   | .binaryApp .getTag x₁ x₂ _
   | .binaryApp .hasTag x₁ x₂ _ =>
     (n > 0) &&
-    (typedAtLevel x₁ (n - 1)) &&
-    (typedAtLevel x₂ n)
+    (checkLevel x₁ (n - 1)) &&
+    (checkLevel x₂ n)
   | .and x₁ x₂ _ -- TODO: Should `and` and `or` take advantage of short-circuiting or is that fully handled in typechecking?
   | .or x₁ x₂ _
   | .binaryApp _ x₁ x₂ _ =>
-    (typedAtLevel x₁ n) &&
-    (typedAtLevel x₂ n)
+    (checkLevel x₁ n) &&
+    (checkLevel x₂ n)
   | .hasAttr x₁ _ _
   | .getAttr x₁ _ _ =>
     match x₁.typeOf with
     | .entity _ =>
       (n > 0) &&
-      (typedAtLevel x₁ (n - 1))
-    | _ => (typedAtLevel x₁ n)
+      (checkLevel x₁ (n - 1))
+    | _ => (checkLevel x₁ n)
   | .call _ xs _
   | .set xs _ =>
     xs.attach.all λ ex =>
-      have : sizeOf ex.val < sizeOf xs := List.sizeOf_lt_of_mem ex.property
-      typedAtLevel ex n
+      have := List.sizeOf_lt_of_mem ex.property
+      checkLevel ex n
   | .record axs _ =>
     axs.attach.all λ a =>
       have : sizeOf a.val.snd < sizeOf axs := by
         have h₁ := List.sizeOf_lt_of_mem a.property
         rw [Prod.mk.sizeOf_spec a.val.fst a.val.snd] at h₁
         omega
-      typedAtLevel a.val.snd n
-  termination_by tx
+      checkLevel a.val.snd n
+
+def typedAtLevel (e : Expr) (c : Capabilities) (env : Environment) (n : Nat) : Bool :=
+  match typeOf e c env with
+  | .ok (te, _) => checkLevel te n
+  | _           => false
