cedar-lean/Cedar/Spec/Slice.lean
@@ -1,0 +1,70 @@
+/-
+ Copyright Cedar Contributors
+
+ Licensed under the Apache License, Version 2.0 (the "License");
+ you may not use this file except in compliance with the License.
+ You may obtain a copy of the License at
+
+      https://www.apache.org/licenses/LICENSE-2.0
+
+ Unless required by applicable law or agreed to in writing, software
+ distributed under the License is distributed on an "AS IS" BASIS,
+ WITHOUT WARRANTIES OR CONDITIONS OF ANY KIND, either express or implied.
+ See the License for the specific language governing permissions and
+ limitations under the License.
+-/
+
+import Cedar.Spec.Value
+import Cedar.Spec.Entities
+import Cedar.Spec.Request
+import Cedar.Data.SizeOf
+
+/-!
+This file defines Cedar entities.
+-/
+
+namespace Cedar.Spec
+
+open Cedar.Data
+
+def flatten_union {α} [LT α] [DecidableLT α] : List (Set α) → Set α :=
+  List.foldl (· ∪ ·) ∅
+
+def Value.sliceEUIDs (v : Value) : Set EntityUID :=
+  match v with
+  | .prim (.entityUID uid) => Set.singleton uid
+  -- TODO: You can't access these except by `in`, so maybe this could just be `Set.empty`
+  | .set s => flatten_union $ s.elts.attach.map λ e => e.val.sliceEUIDs
+  | .record r => flatten_union $ r.toList.attach.map λ e => e.val.snd.sliceEUIDs
+  | .prim _ | .ext _ => ∅
+  decreasing_by
+    · simp [←Nat.succ_eq_one_add, Nat.lt.step, Set.sizeOf_lt_of_mem e.property]
+    · simp only [Map.toList] at e
+      have _ := Map.sizeOf_lt_of_kvs r
+      have _ := List.sizeOf_lt_of_mem e.property
+      have _ : sizeOf e.val.snd < sizeOf e.val := by simp [sizeOf, Prod._sizeOf_1, Nat.one_add]
+      rw [record.sizeOf_spec] ; omega
+
+def EntityData.sliceEUIDs (ed : EntityData) : Set EntityUID :=
+  (flatten_union $ ed.attrs.values.map Value.sliceEUIDs) ∪
+  (flatten_union $ ed.tags.values.map Value.sliceEUIDs)
+
+def Request.sliceEUIDs (r : Request) : Set EntityUID :=
+  Set.make [r.principal, r.action, r.resource] ∪
+  (Value.record r.context).sliceEUIDs
+
+def Entities.sliceAtLevel (es : Entities) (r : Request) (level : Nat) : Option Entities := do
+  Map.make $ ← sliceAtLevel es r.sliceEUIDs r level
+where
+  sliceAtLevel (es : Entities) (work : Set EntityUID) (r : Request) (level : Nat) : Option (List (EntityUID × EntityData)) :=
+    if level == 0 then
+      .some []
+    else do
+      let eds ← work.elts.mapM λ uid => do .some (uid, ←(es.find? uid))
+      let work := flatten_union $ eds.map λ (_, ed) => ed.sliceEUIDs
+      eds ++ (← sliceAtLevel es work r (level - 1))
+    termination_by level
+    decreasing_by
+      rename_i h₁
+      simp only [beq_iff_eq] at h₁
+      omega
