cedar-lean/Cedar/Thm/Validation/Levels.lean
@@ -1,0 +1,317 @@
+/-
+ Copyright Cedar Contributors
+
+ Licensed under the Apache License, Version 2.0 (the "License");
+ you may not use this file except in compliance with the License.
+ You may obtain a copy of the License at
+
+      https://www.apache.org/licenses/LICENSE-2.0
+
+ Unless required by applicable law or agreed to in writing, software
+ distributed under the License is distributed on an "AS IS" BASIS,
+ WITHOUT WARRANTIES OR CONDITIONS OF ANY KIND, either express or implied.
+ See the License for the specific language governing permissions and
+ limitations under the License.
+-/
+
+import Cedar.Spec
+import Cedar.Data
+import Cedar.Validation
+import Cedar.Thm.Validation.Typechecker.IfThenElse
+import Cedar.Thm.Validation.Typechecker
+import Cedar.Thm.Validation.Typechecker.Types
+
+namespace Cedar.Thm
+
+open Cedar.Data
+open Cedar.Spec
+open Cedar.Validation
+
+/-
+theorem lit_level_based_slicing_is_sound {p : Prim} {env : Environment} {request : Request} {entities slice : Entities} {n : Nat} :
+  typedAtLevel (.lit p) env n →
+  slice = entities.sliceAtLevel request n →
+  evaluate (.lit p) request entities = evaluate (.lit p) request slice
+:= by simp [evaluate]
+-/
+
+/-
+theorem check_level_inversion_if {i t e : TypedExpr} {ty : CedarType} {n : Nat} :
+  checkLevel (.ite i t e ty) n →
+  checkLevel i n ∧ checkLevel t n ∧ checkLevel e n
+:= by
+  intros h₁
+  simp [checkLevel] at h₁
+  simp [h₁]
+  -/
+
+--theorem typed_at_level_inversion_if_true {i t e : Expr} {env : Environment} {n : Nat} {c : Capabilities} :
+--  typedAtLevel (.ite i t e) env n →
+--  (typeOf i ∅ env).typeOf = .ok (.bool .tt, c) →
+--  typedAtLevel i env n ∧
+--  typedAtLevel t env n ∧
+--  typedAtLevel e env n
+--:= by
+--  intros h₁ h₂
+--  simp [ResultType.typeOf, Except.map] at h₂
+--  cases h₃ : typeOf i [] env <;> simp [h₃] at h₂
+--  replace ⟨ h₂, h₄ ⟩ := h₂
+--  subst h₄
+--  simp [typedAtLevel, typeOf] at h₁
+--  simp [h₃, bind, Except.bind] at h₁
+--  split at h₁ <;> try contradiction
+
+theorem typed_at_level_then_type_and_level {e : Expr} {c₀: Capabilities} {env : Environment} {n : Nat} :
+  typedAtLevel e c₀ env n ->
+  ∃ tx c₁, typeOf e c₀ env = .ok (tx, c₁) ∧ checkLevel tx n
+:= by
+  unfold typedAtLevel
+  split
+  · rename_i h₂
+    rw [h₂]
+    simp
+  · simp
+
+theorem type_and_level_then_typed_at_level {e : Expr} {tx : TypedExpr} {c₀ c₁: Capabilities} {env : Environment} {n : Nat} :
+  typeOf e c₀ env = .ok (tx, c₁) → checkLevel tx n →
+  typedAtLevel e c₀ env n
+:= by
+  intros h₁
+  unfold typedAtLevel
+  rw [h₁]
+  simp
+
+-- theorem evaluates_to_then_evaluates {e : Expr} {request : Request} {entities slice : Entities} {v : Value} :
+--   slice = entities.sliceAtLevel request n →
+--   EvaluatesTo e request entities v → EvaluatesTo e request slice v →
+--   evaluate e request entities = evaluate e request slice
+-- := by
+--   intros h₁ h₂ h₃
+--   cases e
+--   case lit => simp [evaluate]
+--   case var v => cases v <;> simp [evaluate]
+--   case ite c t e =>
+--     simp [evaluate]
+--     simp [EvaluatesTo, evaluate] at h₂ h₃
+
+
+    -- rcases h₄ : Result.as Bool (evaluate c request entities) with (_ | _) | (_ | _ ) <;>
+    -- rcases h₅ : Result.as Bool (evaluate c request slice) with (_ | _) | (_ | _ ) <;>
+    -- simp [*] at *
+
+
+
+
+
+
+    -- rcases h₅ : Result.as Bool (evaluate c request slice) with _ | _ | _ <;>
+    -- rw [h₄] at h₂ <;>
+    -- rw [h₅] at h₃ <;>
+    -- simp [*] at *
+    -- ·
+
+theorem level_based_slicing_is_sound_zero {e : Expr} {c : Capabilities} {env : Environment} {request : Request} {entities : Entities} :
+  -- slice = entities.sliceAtLevel request 0 →
+  CapabilitiesInvariant c request entities →
+  RequestAndEntitiesMatchEnvironment env request entities →
+  typedAtLevel e c env 0 →
+  evaluate e request entities = evaluate e request Map.empty
+:= by
+  intros hc h₂ h₁
+  have ⟨tx, c', h₃, h₄⟩ := typed_at_level_then_type_and_level h₁
+  cases e
+  case lit => simp [evaluate]
+  case var v => cases v <;> simp [evaluate]
+  case ite c t e =>
+    have ⟨ty₁, bty₁, c₁, ty₂, c₂, ty₃, c₃, h₅, h₆, h₇ ⟩ := type_of_ite_inversion h₃
+    have ⟨ hgc, v, h₁₃, h₁₄ ⟩ := type_of_is_sound hc h₂ h₅
+    rw [h₆] at h₁₄
+    split at h₇
+    · replace ⟨h₇, h₈, _⟩ := h₇
+      subst h₈
+      replace h₁₄ := instance_of_ff_is_false h₁₄
+      subst h₁₄
+      simp only [checkLevel, Bool.and_eq_true] at h₄
+      have ⟨hl₄, hr₄⟩ := h₄
+      have ih₁ := level_based_slicing_is_sound_zero hc h₂ (type_and_level_then_typed_at_level h₇ hr₄)
+      have ih₂ := level_based_slicing_is_sound_zero hc h₂ (type_and_level_then_typed_at_level h₅ hl₄)
+      simp only [evaluate]
+      rw [ih₁, ih₂]
+      cases h₁₂ : Result.as Bool (evaluate c request Map.empty) <;> simp only [Except.bind_err, Except.bind_ok]
+      simp only [Result.as, Coe.coe, Value.asBool] at h₁₂
+      split at h₁₂ <;> try simp at h₁₂
+      split at h₁₂ <;> try simp at h₁₂
+      subst h₁₂
+      rename_i h₁₅
+      unfold EvaluatesTo at h₁₃
+      rw [ih₂, h₁₅] at h₁₃
+      simp only [reduceCtorEq, Except.ok.injEq, Value.prim.injEq, Prim.bool.injEq, false_or] at h₁₃
+      subst h₁₃
+      simp
+    · replace ⟨h₇, h₈, _⟩ := h₇
+      subst h₈ c'
+      replace h₁₄ := instance_of_tt_is_true h₁₄
+      subst h₁₄
+      simp only [checkLevel, Bool.and_eq_true] at h₄
+      have ⟨hl₄, hr₄⟩ := h₄ ; clear h₄
+      have ih₂ := level_based_slicing_is_sound_zero hc h₂ (type_and_level_then_typed_at_level h₅ hl₄)
+      simp only [evaluate]
+      rw [ih₂]
+      cases h₁₂ : Result.as Bool (evaluate c request Map.empty) <;> simp only [Except.bind_err, Except.bind_ok]
+      simp only [Result.as, Coe.coe, Value.asBool] at h₁₂
+      split at h₁₂ <;> try simp at h₁₂
+      split at h₁₂ <;> try simp at h₁₂
+      subst h₁₂
+      rename_i h₁₅
+      unfold EvaluatesTo at h₁₃
+      rw [ih₂, h₁₅] at h₁₃
+      simp only [reduceCtorEq, Except.ok.injEq, Value.prim.injEq, Prim.bool.injEq, false_or] at h₁₃
+      subst h₁₃
+      simp [GuardedCapabilitiesInvariant] at hgc
+      rw [ih₂, h₁₅] at hgc
+      simp at hgc
+      have ih₁ := level_based_slicing_is_sound_zero (capability_union_invariant hc hgc) h₂ (type_and_level_then_typed_at_level h₇ hr₄)
+      rw [ih₁]
+      simp
+    · replace ⟨h₇, h₈, h₉, h₁₀, _⟩ := h₇
+      rw [h₉] at h₄
+      simp only [checkLevel, Bool.and_eq_true] at h₄
+      have ⟨⟨ ha₄, hb₄ ⟩, hc₄ ⟩ := h₄
+      have ih₁ := level_based_slicing_is_sound_zero hc h₂ (type_and_level_then_typed_at_level h₅ ha₄)
+      have ih₃ := level_based_slicing_is_sound_zero hc h₂ (type_and_level_then_typed_at_level h₈ hc₄)
+      simp only [evaluate]
+      rw [ih₁, ih₃]
+      cases h₁₂ : Result.as Bool (evaluate c request Map.empty) <;> simp only [Except.bind_err, Except.bind_ok]
+      simp only [Result.as, Coe.coe, Value.asBool] at h₁₂
+      split at h₁₂ <;> try simp at h₁₂
+      split at h₁₂ <;> try simp at h₁₂
+      subst h₁₂
+      rename_i h₁₄
+      unfold EvaluatesTo at h₁₃
+      rw [ih₁, h₁₄] at h₁₃
+      simp only [reduceCtorEq, Except.ok.injEq, false_or] at h₁₃
+      rename_i b
+      cases b
+      case false => simp
+      case true =>
+        simp only [GuardedCapabilitiesInvariant, ih₁, h₁₄, forall_const] at hgc
+        have ih₂ := level_based_slicing_is_sound_zero (capability_union_invariant hc hgc) h₂ (type_and_level_then_typed_at_level h₇ hb₄)
+        simp [ih₂]
+
+  case and => sorry
+  case or => sorry
+  case unaryApp => sorry
+  case binaryApp => sorry
+  case getAttr => sorry
+  case hasAttr => sorry
+  case set => sorry
+  case record => sorry
+  case call => sorry
+
+
+
+
+-- theorem level_based_slicing_is_sound' {e : Expr} {env : Environment} {request : Request} {entities slice : Entities} {n : Nat} :
+--   slice = entities.sliceAtLevel request n →
+--   typedAtLevel e env n →
+--   evaluate e request entities = evaluate e request slice
+-- := by
+--   intros h₁ h₂
+--   cases n
+--   ·
+--     simp [Entities.sliceAtLevel, Entities.sliceAtLevel.sliceAtLevel, Map.make, List.canonicalize] at h₁
+--     subst slice
+--     simp [typedAtLevel] at h₂
+--     split at h₂ <;> try simp at h₂
+--     -- unfold checkLevel at h₂
+
+
+
+/-
+theorem level_based_slicing_is_sound {e : Expr} {env : Environment} {request : Request} {entities slice : Entities} {n : Nat} :
+  slice = entities.sliceAtLevel request n →
+  typedAtLevel e env n →
+  evaluate e request entities = evaluate e request slice
+:= by
+  intros h₁
+  cases e
+  case lit =>
+    simp [evaluate]
+  case var v =>
+    cases v <;> simp [evaluate]
+  case ite c t e =>
+    intros h₂
+    have ⟨_, _, h₃, h₄⟩ := typed_at_level_then_type_and_level h₂
+    have ⟨ty₁, bty₁, c₁, ty₂, c₂, ty₃, c₃, h₅, h₆, h₇ ⟩  := type_of_ite_inversion h₃
+    split at h₇
+    · replace ⟨h₇, h₈, h₉⟩ := h₇
+      subst c₃ ty₃
+      have h₁₀ : typedAtLevel e env n := by sorry
+      have h₁₁ := level_based_slicing_is_sound h₁ h₁₀
+      have hc := empty_capabilities_invariant request entities
+      have ⟨ hgc, v, h₁₂, h₁₃ ⟩ := type_of_is_sound hc (by sorry) h₅
+      have hc' := empty_capabilities_invariant request slice
+      have ⟨ hgc', v', h'₁₂, h'₁₃ ⟩ := type_of_is_sound hc' (by sorry) h₅
+      rw [h₆] at h₁₃
+      rw [h₆] at h'₁₃
+      have h₁₄ := instance_of_ff_is_false h₁₃
+      have h'₁₄ := instance_of_ff_is_false h'₁₃
+      subst v v'
+      simp [evaluate]
+      cases h₁₂ <;> cases h'₁₂
+      · rename_i h₁₂ h'₁₂
+        rw [h₁₂, h'₁₂]
+        simp [Result.as]
+      · rename_i h₁₂ h'₁₂
+        cases h₁₂ <;> cases h'₁₂
+      · sorry
+      · sorry
+
+
+
+
+
+
+
+
+
+      unfold EvaluatesTo at h₁₂
+
+
+    simp [evaluate]
+    intros h₂
+    simp [typedAtLevel] at h₂
+    split at h₂
+
+
+    cases h₂ : evaluate c request entities <;>
+    cases h₃ : evaluate c request slice <;>
+    simp [Result.as, bind, Except.bind]
+    case error.ok =>
+      unfold typedAtLevel
+      cases h₄ : typeOf (c.ite t e) ∅ env <;> simp
+      intros
+      have ih := level_based_slicing_is_sound h₁
+
+
+
+    --case error.error =>
+    --  unfold typedAtLevel
+    --  cases h₄ : typeOf (c.ite t e) ∅ env
+    --  case error => simp
+    --  case ok =>
+    --    simp ; intros
+
+
+
+  case and => sorry
+  case or => sorry
+  case unaryApp => sorry
+  case binaryApp => sorry
+  case getAttr => sorry
+  case hasAttr => sorry
+  case set => sorry
+  case record => sorry
+  case call => sorry
+
+-/
