cedar-lean/Cedar/Thm/Validation/Typechecker/IfThenElse.lean
@@ -27,27 +27,28 @@ open Cedar.Validation
 
 theorem type_of_ite_inversion {x₁ x₂ x₃ : Expr} {c c' : Capabilities} {env : Environment} {ty : TypedExpr}
   (h₁ : typeOf (Expr.ite x₁ x₂ x₃) c env = Except.ok (ty, c')) :
-  ∃ bty₁ c₁ ty₂ c₂ ty₃ c₃,
-    (typeOf x₁ c env).typeOf = .ok (.bool bty₁, c₁) ∧
+  ∃ ty₁ bty₁ c₁ ty₂ c₂ ty₃ c₃,
+    typeOf x₁ c env = .ok (ty₁, c₁) ∧
+    ty₁.typeOf = .bool bty₁ ∧
     match bty₁ with
     | .ff      =>
-      typeOf x₃ c env = .ok (ty₃, c₃) ∧ ty = ty₃ ∧ c' = c₃
+      typeOf x₃ c env = .ok (ty₃, c₃) ∧ ty = TypedExpr.and (TypedExpr.unaryApp .not ty₁ (.bool .tt)) ty₃ ty₃.typeOf ∧ c' = c₃
     | .tt      =>
       typeOf x₂ (c ∪ c₁) env = .ok (ty₂, c₂) ∧
-      ty = ty₂ ∧ c' = c₁ ∪ c₂
+      ty = TypedExpr.and ty₁ ty₂ ty₂.typeOf ∧ c' = c₁ ∪ c₂
     | .anyBool =>
       typeOf x₂ (c ∪ c₁) env = .ok (ty₂, c₂) ∧
       typeOf x₃ c env = .ok (ty₃, c₃) ∧
+      ty = TypedExpr.ite ty₁ ty₂ ty₃ ty.typeOf ∧
       (ty₂.typeOf ⊔ ty₃.typeOf) = (.some ty.typeOf) ∧ c' = (c₁ ∪ c₂) ∩ c₃
 := by
   simp [typeOf] at h₁
   cases h₂ : typeOf x₁ c env <;> simp [h₂, typeOfIf] at *
-  simp [ResultType.typeOf, Except.map]
   rename_i res₁
   split at h₁ <;> try { simp [ok, err] at h₁ } <;>
   rename_i c₁ hr₁
   case ok.h_1 =>
-    exists BoolType.tt, res₁.snd
+    exists res₁.fst, BoolType.tt, res₁.snd
     simp [hr₁]
     cases h₃ : typeOf x₂ (c ∪ res₁.snd) env <;> simp [h₃] at h₁
     rename_i res₂ ; simp [ok] at h₁
@@ -56,11 +57,16 @@ theorem type_of_ite_inversion {x₁ x₂ x₃ : Expr} {c c' : Capabilities} {env
     subst ht₂ hc₂
     simp [h₃, ←hr₁]
   case ok.h_2 =>
-    exists BoolType.ff, res₁.snd
+    exists res₁.fst, BoolType.ff, res₁.snd
     simp [hr₁]
-    exact h₁
+    cases h₃ : typeOf x₃ c env <;> simp [h₃] at h₁
+    rename_i res₃
+    simp [ok] at h₁
+    replace ⟨hl₁, hr₁⟩ := h₁
+    subst hl₁ hr₁
+    exists res₃.fst
   case ok.h_3 =>
-    exists BoolType.anyBool, res₁.snd
+    exists res₁.fst, BoolType.anyBool, res₁.snd
     simp [hr₁]
     cases h₃ : typeOf x₂ (c ∪ res₁.snd) env <;> simp [h₃] at h₁
     cases h₄ : typeOf x₃ c env <;> simp [h₄] at h₁
@@ -82,16 +88,15 @@ theorem type_of_ite_is_sound {x₁ x₂ x₃ : Expr} {c₁ c₂ : Capabilities} 
   GuardedCapabilitiesInvariant (Expr.ite x₁ x₂ x₃) c₂ request entities ∧
   ∃ v, EvaluatesTo (Expr.ite x₁ x₂ x₃) request entities v ∧ InstanceOfType v ty.typeOf
 := by
-  have ⟨bty₁, rc₁, ty₂, rc₂, ty₃, rc₃, h₄, h₅⟩ := type_of_ite_inversion h₃
-  split_type_of h₄ ; rename_i h₄ hl₄ hr₄
+  have ⟨ty₁, bty₁, rc₁, ty₂, rc₂, ty₃, rc₃, h₄, h₅, h₆⟩ := type_of_ite_inversion h₃
   specialize ih₁ h₁ h₂ h₄
   have ⟨ih₁₁, v₁, ih₁₂, ih₁₃⟩ := ih₁
-  simp [hl₄] at ih₁₃
+  simp [h₅] at ih₁₃
   have ⟨b₁, hb₁⟩ := instance_of_bool_is_bool ih₁₃
   subst hb₁
-  cases bty₁ <;> simp at h₅
+  cases bty₁ <;> simp at h₆
   case anyBool =>
-    have ⟨h₅, h₆, ht, hc⟩ := h₅
+    have ⟨h₅, h₆, ht, hty, hc⟩ := h₆
     cases b₁
     case false =>
       rcases ih₁₂ with ih₁₂ | ih₁₂ | ih₁₂ | ih₁₂ <;>
@@ -108,7 +113,7 @@ theorem type_of_ite_is_sound {x₁ x₂ x₃ : Expr} {c₁ c₂ : Capabilities} 
         apply capability_intersection_invariant
         simp [ih₃₁]
       case right =>
-        apply instance_of_lub ht
+        apply instance_of_lub hty
         simp [ih₃₃]
     case true =>
       rcases ih₁₂ with ih₁₂ | ih₁₂ | ih₁₂ | ih₁₂ <;>
@@ -116,7 +121,6 @@ theorem type_of_ite_is_sound {x₁ x₂ x₃ : Expr} {c₁ c₂ : Capabilities} 
       try exact type_is_inhabited ty.typeOf
       simp [GuardedCapabilitiesInvariant, ih₁₂] at ih₁₁
       have h₇ := capability_union_invariant h₁ ih₁₁
-      subst rc₁
       specialize ih₂ h₇ h₂ h₅
       have ⟨ih₂₁, v₂, ih₂₂, ih₂₃⟩ := ih₂
       apply And.intro
@@ -130,10 +134,10 @@ theorem type_of_ite_is_sound {x₁ x₂ x₃ : Expr} {c₁ c₂ : Capabilities} 
       case right =>
         rcases ih₂₂ with ih₂₂ | ih₂₂ | ih₂₂ | ih₂₂ <;> simp [ih₂₂] <;>
         try exact type_is_inhabited ty.typeOf
-        apply instance_of_lub ht
+        apply instance_of_lub hty
         simp [ih₂₃]
   case tt =>
-    have ⟨h₅, ht, hc⟩ := h₅
+    have ⟨h₅, ht, hc⟩ := h₆
     rcases ih₁₂ with ih₁₂ | ih₁₂ | ih₁₂ | ih₁₂ <;>
     simp [EvaluatesTo, evaluate, Result.as, ih₁₂, Coe.coe, Value.asBool, GuardedCapabilitiesInvariant] <;>
     try exact type_is_inhabited ty.typeOf
@@ -141,17 +145,18 @@ theorem type_of_ite_is_sound {x₁ x₂ x₃ : Expr} {c₁ c₂ : Capabilities} 
     simp at hb₁ ; subst hb₁ ; simp only [ite_true]
     simp [GuardedCapabilitiesInvariant, ih₁₂] at ih₁₁
     have h₆ := capability_union_invariant h₁ ih₁₁
-    subst rc₁
     specialize ih₂ h₆ h₂ h₅
     have ⟨ih₂₁, v₂, ih₂₂, ih₂₃⟩ := ih₂
     rcases ih₂₂ with ih₂₂ | ih₂₂ | ih₂₂ | ih₂₂ <;> simp [ih₂₂] <;>
     try exact type_is_inhabited ty.typeOf
-    subst ht hc ; simp [ih₂₃]
+    unfold TypedExpr.typeOf
+    subst ht hc
+    simp [ih₂₃]
     intro h₇ ; subst h₇
     simp [GuardedCapabilitiesInvariant, ih₂₂] at ih₂₁
     exact capability_union_invariant ih₁₁ ih₂₁
   case ff =>
-    have ⟨h₅, ht, hc⟩ := h₅
+    have ⟨h₅, ht, hc⟩ := h₆
     rcases ih₁₂ with ih₁₂ | ih₁₂ | ih₁₂ | ih₁₂ <;>
     simp [EvaluatesTo, evaluate, Result.as, ih₁₂, Coe.coe, Value.asBool, GuardedCapabilitiesInvariant] <;>
     try exact type_is_inhabited ty.typeOf
