cedar-lean/Cedar/Validation/Typechecker.lean
@@ -76,8 +76,11 @@ def typeOfIf (r₁ : TypedExpr × Capabilities) (r₂ r₃ : ResultType) : Resul
   match r₁.fst.typeOf with
   | .bool .tt  => do
     let (ty₂, c₂) ← r₂
-    ok ty₂ (c₁ ∪ c₂)
-  | .bool .ff => r₃
+    -- Changed during proof of slicing soundness. Previously returned ty₂ directly
+    ok (.and r₁.fst ty₂ ty₂.typeOf) (c₁ ∪ c₂)
+  | .bool .ff => do
+    let (ty₃, c₃) ← r₃
+    ok (.and (.unaryApp .not r₁.fst (.bool .tt)) ty₃ ty₃.typeOf) c₃
   | .bool .anyBool => do
     let (ty₂, c₂) ← r₂
     let (ty₃, c₃) ← r₃
